jwnlgj

.lake/build/ir/Games/gameLib/Basic.c
@@ -13,73 +13,61 @@
 #ifdef __cplusplus
 extern "C" {
 #endif
-LEAN_EXPORT lean_object* l_Symm__Game__World_hist__on__turn___at_Symm__Game_hist__on__turn___spec__1___rarg(lean_object*, lean_object*, lean_object*, lean_object*, lean_object*, lean_object*);
 LEAN_EXPORT lean_object* l_instDecidablePredListHist__neutral(lean_object*, lean_object*, lean_object*);
-LEAN_EXPORT lean_object* l_Symm__Game_hist__on__turn___rarg(lean_object*, lean_object*, lean_object*, lean_object*);
-LEAN_EXPORT lean_object* l_Game__World_state__on__turn___rarg(lean_object*, lean_object*, lean_object*, lean_object*, lean_object*, lean_object*);
+LEAN_EXPORT lean_object* l_Symm__Game_hist__on__turn___rarg(lean_object*, lean_object*);
+LEAN_EXPORT lean_object* l_Game__World_state__on__turn___rarg(lean_object*, lean_object*, lean_object*, lean_object*);
+LEAN_EXPORT lean_object* l_Symm__Game_hist__on__turn___rarg___boxed(lean_object*, lean_object*);
+LEAN_EXPORT lean_object* l_Symm__Game_state__on__turn___rarg___boxed(lean_object*, lean_object*);
 LEAN_EXPORT lean_object* l_instDecidablePredListHist__legal(lean_object*, lean_object*, lean_object*);
-LEAN_EXPORT lean_object* l_Symm__Game__World_hist__on__turn___rarg(lean_object*, lean_object*, lean_object*, lean_object*, lean_object*, lean_object*);
+LEAN_EXPORT lean_object* l_Symm__Game__World_hist__on__turn___rarg(lean_object*, lean_object*, lean_object*, lean_object*);
 LEAN_EXPORT lean_object* l_Symm__Game__World_state__on__turn(lean_object*, lean_object*);
 LEAN_EXPORT lean_object* l_instDecidablePredListHist__legal___rarg___lambda__1___boxed(lean_object*, lean_object*, lean_object*, lean_object*, lean_object*);
-LEAN_EXPORT lean_object* l_Game__World__wDraw_hist__on__turn___rarg(lean_object*, lean_object*, lean_object*, lean_object*, lean_object*, lean_object*);
-LEAN_EXPORT lean_object* l_Game__World__wDraw_hist__on__turn___rarg___boxed(lean_object*, lean_object*, lean_object*, lean_object*, lean_object*, lean_object*);
-LEAN_EXPORT lean_object* l_Game_state__on__turn___rarg(lean_object*, lean_object*, lean_object*, lean_object*);
+LEAN_EXPORT lean_object* l_Game__World__wDraw_hist__on__turn___rarg(lean_object*, lean_object*, lean_object*, lean_object*);
+LEAN_EXPORT lean_object* l_Game__World__wDraw_hist__on__turn___rarg___boxed(lean_object*, lean_object*, lean_object*, lean_object*);
+LEAN_EXPORT lean_object* l_Game_state__on__turn___rarg(lean_object*, lean_object*);
 static lean_object* l_instCoeSymm__Game__WorldGame__World___closed__1;
-LEAN_EXPORT lean_object* l_Game_hist__on__turn___rarg___boxed(lean_object*, lean_object*, lean_object*, lean_object*);
+LEAN_EXPORT lean_object* l_Game_hist__on__turn___rarg___boxed(lean_object*, lean_object*);
 lean_object* l_List_rec____x40_Mathlib_Util_CompileInductive___hyg_3246____rarg(lean_object*, lean_object*, lean_object*);
 LEAN_EXPORT lean_object* l_Symm__Game__World_toGame__World___elambda__1(lean_object*, lean_object*);
-LEAN_EXPORT lean_object* l_Game__World_state__on__turn___at_Game_state__on__turn___spec__1___boxed(lean_object*, lean_object*, lean_object*);
-LEAN_EXPORT lean_object* l_Symm__Game__World_hist__on__turn___at_Symm__Game_hist__on__turn___spec__1(lean_object*, lean_object*, lean_object*);
 LEAN_EXPORT lean_object* l_Symm__Game_toGame___rarg(lean_object*);
-LEAN_EXPORT lean_object* l_Game__World_state__on__turn___at_Symm__Game_state__on__turn___spec__2___boxed(lean_object*, lean_object*, lean_object*);
 uint8_t l_instDecidablePredNatTurn__fst(lean_object*);
-LEAN_EXPORT lean_object* l_Game__World_hist__on__turn___rarg(lean_object*, lean_object*, lean_object*, lean_object*, lean_object*, lean_object*);
+LEAN_EXPORT lean_object* l_Game__World_hist__on__turn___rarg(lean_object*, lean_object*, lean_object*, lean_object*);
 LEAN_EXPORT lean_object* l_instDecidablePredListHist__neutral___boxed(lean_object*, lean_object*, lean_object*);
+LEAN_EXPORT lean_object* l_Game_state__on__turn___rarg___boxed(lean_object*, lean_object*);
 LEAN_EXPORT lean_object* l_Symm__Game_toGame___elambda__2(lean_object*, lean_object*);
-LEAN_EXPORT lean_object* l_Symm__Game_state__on__turn___rarg(lean_object*, lean_object*, lean_object*, lean_object*);
+LEAN_EXPORT lean_object* l_Symm__Game_state__on__turn___rarg(lean_object*, lean_object*);
 LEAN_EXPORT lean_object* l_Game__World__wDraw_hist__on__turn(lean_object*, lean_object*);
-LEAN_EXPORT lean_object* l_Symm__Game__World_state__on__turn___at_Symm__Game_state__on__turn___spec__1___rarg(lean_object*, lean_object*, lean_object*, lean_object*, lean_object*, lean_object*, lean_object*);
 LEAN_EXPORT lean_object* l_Symm__Game__World_toGame__World___elambda__1___rarg(lean_object*, lean_object*, lean_object*);
 lean_object* l_List_lengthTRAux___rarg(lean_object*, lean_object*);
-LEAN_EXPORT lean_object* l_Game__World_state__on__turn___at_Symm__Game_state__on__turn___spec__2(lean_object*, lean_object*, lean_object*);
 LEAN_EXPORT lean_object* l_Symm__Game__World_toGame__World(lean_object*, lean_object*);
-LEAN_EXPORT lean_object* l_Game__World_state__on__turn___at_Symm__Game_state__on__turn___spec__2___rarg(lean_object*, lean_object*, lean_object*, lean_object*, lean_object*, lean_object*);
 LEAN_EXPORT uint8_t l_instDecidablePredListHist__neutral___rarg(lean_object*, lean_object*, lean_object*);
 LEAN_EXPORT lean_object* l_Symm__Game__World_toGame__World___rarg(lean_object*);
 LEAN_EXPORT lean_object* l_Game_hist__on__turn(lean_object*, lean_object*);
-LEAN_EXPORT lean_object* l_Symm__Game__World_state__on__turn___at_Symm__Game_state__on__turn___spec__1___rarg___boxed(lean_object*, lean_object*, lean_object*, lean_object*, lean_object*, lean_object*, lean_object*);
 LEAN_EXPORT lean_object* l_Symm__Game__World_hist__on__turn(lean_object*, lean_object*);
 LEAN_EXPORT lean_object* l_Game__World_state__from__hist(lean_object*, lean_object*);
-LEAN_EXPORT lean_object* l_Game__World_state__on__turn___at_Game_state__on__turn___spec__1(lean_object*, lean_object*, lean_object*);
-LEAN_EXPORT lean_object* l_Symm__Game__World_state__on__turn___at_Symm__Game_state__on__turn___spec__1(lean_object*, lean_object*);
 LEAN_EXPORT lean_object* l_Symm__Game_toGame___elambda__1___rarg(lean_object*, lean_object*, lean_object*, lean_object*);
 LEAN_EXPORT lean_object* l_Symm__Game_toGame___elambda__1(lean_object*, lean_object*);
 uint8_t lean_nat_dec_eq(lean_object*, lean_object*);
-LEAN_EXPORT lean_object* l_Symm__Game__World_hist__on__turn___at_Symm__Game_hist__on__turn___spec__1___boxed(lean_object*, lean_object*, lean_object*);
 LEAN_EXPORT lean_object* l_instDecidablePredListHist__legal___boxed(lean_object*, lean_object*, lean_object*);
 LEAN_EXPORT lean_object* l_Game_state__on__turn(lean_object*, lean_object*);
 LEAN_EXPORT lean_object* l_Symm__Game_state__on__turn(lean_object*, lean_object*);
-LEAN_EXPORT lean_object* l_Game__World_state__on__turn___at_Game_state__on__turn___spec__1___rarg(lean_object*, lean_object*, lean_object*, lean_object*, lean_object*, lean_object*);
 lean_object* lean_nat_sub(lean_object*, lean_object*);
-LEAN_EXPORT lean_object* l_Symm__Game__World_state__on__turn___rarg(lean_object*, lean_object*, lean_object*, lean_object*, lean_object*, lean_object*);
-LEAN_EXPORT lean_object* l_Symm__Game__World_state__on__turn___rarg___boxed(lean_object*, lean_object*, lean_object*, lean_object*, lean_object*, lean_object*);
+LEAN_EXPORT lean_object* l_Symm__Game__World_state__on__turn___rarg(lean_object*, lean_object*, lean_object*, lean_object*);
+LEAN_EXPORT lean_object* l_Symm__Game__World_state__on__turn___rarg___boxed(lean_object*, lean_object*, lean_object*, lean_object*);
 LEAN_EXPORT lean_object* l_Game__World_state__from__hist___rarg(lean_object*, lean_object*);
 LEAN_EXPORT lean_object* l_instDecidablePredListHist__legal___rarg___lambda__1(lean_object*, lean_object*, lean_object*, lean_object*, uint8_t);
-LEAN_EXPORT lean_object* l_Game__World_state__on__turn___at_Symm__Game_state__on__turn___spec__2___rarg___boxed(lean_object*, lean_object*, lean_object*, lean_object*, lean_object*, lean_object*);
 LEAN_EXPORT lean_object* l_Symm__Game_hist__on__turn(lean_object*, lean_object*);
-LEAN_EXPORT lean_object* l_Game__World_state__on__turn___at_Game_state__on__turn___spec__1___rarg___boxed(lean_object*, lean_object*, lean_object*, lean_object*, lean_object*, lean_object*);
 LEAN_EXPORT lean_object* l_Symm__Game_toGame___elambda__2___rarg(lean_object*, lean_object*, lean_object*, lean_object*);
-LEAN_EXPORT lean_object* l_Game__World_hist__on__turn___rarg___boxed(lean_object*, lean_object*, lean_object*, lean_object*, lean_object*, lean_object*);
-LEAN_EXPORT lean_object* l_Symm__Game__World_hist__on__turn___rarg___boxed(lean_object*, lean_object*, lean_object*, lean_object*, lean_object*, lean_object*);
+LEAN_EXPORT lean_object* l_Game__World_hist__on__turn___rarg___boxed(lean_object*, lean_object*, lean_object*, lean_object*);
+LEAN_EXPORT lean_object* l_Symm__Game__World_hist__on__turn___rarg___boxed(lean_object*, lean_object*, lean_object*, lean_object*);
 LEAN_EXPORT lean_object* l_Game__World_state__on__turn(lean_object*, lean_object*);
-LEAN_EXPORT lean_object* l_Game_hist__on__turn___rarg(lean_object*, lean_object*, lean_object*, lean_object*);
+LEAN_EXPORT lean_object* l_Game_hist__on__turn___rarg(lean_object*, lean_object*);
 LEAN_EXPORT lean_object* l_instCoeSymm__Game__WorldGame__World(lean_object*, lean_object*);
 LEAN_EXPORT lean_object* l_Symm__Game_toGame(lean_object*, lean_object*);
 lean_object* lean_nat_add(lean_object*, lean_object*);
 LEAN_EXPORT lean_object* l_instDecidablePredListHist__neutral___rarg___boxed(lean_object*, lean_object*, lean_object*);
-LEAN_EXPORT lean_object* l_Symm__Game__World_hist__on__turn___at_Symm__Game_hist__on__turn___spec__1___rarg___boxed(lean_object*, lean_object*, lean_object*, lean_object*, lean_object*, lean_object*);
 LEAN_EXPORT lean_object* l_instDecidablePredListHist__legal___rarg(lean_object*, lean_object*, lean_object*);
-LEAN_EXPORT lean_object* l_Game__World_state__on__turn___rarg___boxed(lean_object*, lean_object*, lean_object*, lean_object*, lean_object*, lean_object*);
+LEAN_EXPORT lean_object* l_Game__World_state__on__turn___rarg___boxed(lean_object*, lean_object*, lean_object*, lean_object*);
 LEAN_EXPORT lean_object* l_Game__World_hist__on__turn(lean_object*, lean_object*);
 LEAN_EXPORT lean_object* l_Symm__Game__World_toGame__World___elambda__1___rarg(lean_object* x_1, lean_object* x_2, lean_object* x_3) {
 _start:
@@ -285,54 +273,54 @@ lean_dec(x_3);
 return x_4;
 }
 }
-LEAN_EXPORT lean_object* l_Game__World_hist__on__turn___rarg(lean_object* x_1, lean_object* x_2, lean_object* x_3, lean_object* x_4, lean_object* x_5, lean_object* x_6) {
+LEAN_EXPORT lean_object* l_Game__World_hist__on__turn___rarg(lean_object* x_1, lean_object* x_2, lean_object* x_3, lean_object* x_4) {
 _start:
 {
-lean_object* x_7; uint8_t x_8; 
-x_7 = lean_unsigned_to_nat(0u);
-x_8 = lean_nat_dec_eq(x_6, x_7);
-if (x_8 == 0)
+lean_object* x_5; uint8_t x_6; 
+x_5 = lean_unsigned_to_nat(0u);
+x_6 = lean_nat_dec_eq(x_4, x_5);
+if (x_6 == 0)
 {
-lean_object* x_9; lean_object* x_10; lean_object* x_11; lean_object* x_12; uint8_t x_13; 
-x_9 = lean_unsigned_to_nat(1u);
-x_10 = lean_nat_sub(x_6, x_9);
-lean_inc(x_5);
-lean_inc(x_4);
-x_11 = l_Game__World_hist__on__turn___rarg(x_1, x_2, x_3, x_4, x_5, x_10);
-x_12 = lean_nat_add(x_10, x_9);
+lean_object* x_7; lean_object* x_8; lean_object* x_9; lean_object* x_10; uint8_t x_11; 
+x_7 = lean_unsigned_to_nat(1u);
+x_8 = lean_nat_sub(x_4, x_7);
+lean_inc(x_3);
+lean_inc(x_2);
+x_9 = l_Game__World_hist__on__turn___rarg(x_1, x_2, x_3, x_8);
+x_10 = lean_nat_add(x_8, x_7);
+lean_dec(x_8);
+x_11 = l_instDecidablePredNatTurn__fst(x_10);
 lean_dec(x_10);
-x_13 = l_instDecidablePredNatTurn__fst(x_12);
-lean_dec(x_12);
-if (x_13 == 0)
+if (x_11 == 0)
+{
+lean_object* x_12; lean_object* x_13; 
+lean_dec(x_2);
+lean_inc(x_9);
+x_12 = lean_apply_3(x_3, x_9, lean_box(0), lean_box(0));
+x_13 = lean_alloc_ctor(1, 2, 0);
+lean_ctor_set(x_13, 0, x_12);
+lean_ctor_set(x_13, 1, x_9);
+return x_13;
+}
+else
 {
 lean_object* x_14; lean_object* x_15; 
-lean_dec(x_4);
-lean_inc(x_11);
-x_14 = lean_apply_3(x_5, x_11, lean_box(0), lean_box(0));
+lean_dec(x_3);
+lean_inc(x_9);
+x_14 = lean_apply_3(x_2, x_9, lean_box(0), lean_box(0));
 x_15 = lean_alloc_ctor(1, 2, 0);
 lean_ctor_set(x_15, 0, x_14);
-lean_ctor_set(x_15, 1, x_11);
+lean_ctor_set(x_15, 1, x_9);
 return x_15;
 }
-else
-{
-lean_object* x_16; lean_object* x_17; 
-lean_dec(x_5);
-lean_inc(x_11);
-x_16 = lean_apply_3(x_4, x_11, lean_box(0), lean_box(0));
-x_17 = lean_alloc_ctor(1, 2, 0);
-lean_ctor_set(x_17, 0, x_16);
-lean_ctor_set(x_17, 1, x_11);
-return x_17;
-}
 }
 else
 {
-lean_object* x_18; 
-lean_dec(x_5);
-lean_dec(x_4);
-x_18 = lean_box(0);
-return x_18;
+lean_object* x_16; 
+lean_dec(x_3);
+lean_dec(x_2);
+x_16 = lean_box(0);
+return x_16;
 }
 }
 }
@@ -340,77 +328,71 @@ LEAN_EXPORT lean_object* l_Game__World_hist__on__turn(lean_object* x_1, lean_obj
 _start:
 {
 lean_object* x_3; 
-x_3 = lean_alloc_closure((void*)(l_Game__World_hist__on__turn___rarg___boxed), 6, 0);
+x_3 = lean_alloc_closure((void*)(l_Game__World_hist__on__turn___rarg___boxed), 4, 0);
 return x_3;
 }
 }
-LEAN_EXPORT lean_object* l_Game__World_hist__on__turn___rarg___boxed(lean_object* x_1, lean_object* x_2, lean_object* x_3, lean_object* x_4, lean_object* x_5, lean_object* x_6) {
+LEAN_EXPORT lean_object* l_Game__World_hist__on__turn___rarg___boxed(lean_object* x_1, lean_object* x_2, lean_object* x_3, lean_object* x_4) {
 _start:
 {
-lean_object* x_7; 
-x_7 = l_Game__World_hist__on__turn___rarg(x_1, x_2, x_3, x_4, x_5, x_6);
-lean_dec(x_6);
-lean_dec(x_3);
-lean_dec(x_2);
+lean_object* x_5; 
+x_5 = l_Game__World_hist__on__turn___rarg(x_1, x_2, x_3, x_4);
+lean_dec(x_4);
 lean_dec(x_1);
-return x_7;
+return x_5;
 }
 }
-LEAN_EXPORT lean_object* l_Symm__Game__World_hist__on__turn___rarg(lean_object* x_1, lean_object* x_2, lean_object* x_3, lean_object* x_4, lean_object* x_5, lean_object* x_6) {
+LEAN_EXPORT lean_object* l_Symm__Game__World_hist__on__turn___rarg(lean_object* x_1, lean_object* x_2, lean_object* x_3, lean_object* x_4) {
 _start:
 {
-lean_object* x_7; lean_object* x_8; 
-x_7 = l_Symm__Game__World_toGame__World___rarg(x_1);
-x_8 = l_Game__World_hist__on__turn___rarg(x_7, x_2, x_3, x_4, x_5, x_6);
-lean_dec(x_7);
-return x_8;
+lean_object* x_5; lean_object* x_6; 
+x_5 = l_Symm__Game__World_toGame__World___rarg(x_1);
+x_6 = l_Game__World_hist__on__turn___rarg(x_5, x_2, x_3, x_4);
+lean_dec(x_5);
+return x_6;
 }
 }
 LEAN_EXPORT lean_object* l_Symm__Game__World_hist__on__turn(lean_object* x_1, lean_object* x_2) {
 _start:
 {
 lean_object* x_3; 
-x_3 = lean_alloc_closure((void*)(l_Symm__Game__World_hist__on__turn___rarg___boxed), 6, 0);
+x_3 = lean_alloc_closure((void*)(l_Symm__Game__World_hist__on__turn___rarg___boxed), 4, 0);
 return x_3;
 }
 }
-LEAN_EXPORT lean_object* l_Symm__Game__World_hist__on__turn___rarg___boxed(lean_object* x_1, lean_object* x_2, lean_object* x_3, lean_object* x_4, lean_object* x_5, lean_object* x_6) {
+LEAN_EXPORT lean_object* l_Symm__Game__World_hist__on__turn___rarg___boxed(lean_object* x_1, lean_object* x_2, lean_object* x_3, lean_object* x_4) {
 _start:
 {
-lean_object* x_7; 
-x_7 = l_Symm__Game__World_hist__on__turn___rarg(x_1, x_2, x_3, x_4, x_5, x_6);
-lean_dec(x_6);
-lean_dec(x_3);
-lean_dec(x_2);
-return x_7;
+lean_object* x_5; 
+x_5 = l_Symm__Game__World_hist__on__turn___rarg(x_1, x_2, x_3, x_4);
+lean_dec(x_4);
+return x_5;
 }
 }
-LEAN_EXPORT lean_object* l_Game__World__wDraw_hist__on__turn___rarg(lean_object* x_1, lean_object* x_2, lean_object* x_3, lean_object* x_4, lean_object* x_5, lean_object* x_6) {
+LEAN_EXPORT lean_object* l_Game__World__wDraw_hist__on__turn___rarg(lean_object* x_1, lean_object* x_2, lean_object* x_3, lean_object* x_4) {
 _start:
 {
-lean_object* x_7; 
-x_7 = l_Game__World_hist__on__turn___rarg(x_1, x_2, x_3, x_4, x_5, x_6);
-return x_7;
+lean_object* x_5; 
+x_5 = l_Game__World_hist__on__turn___rarg(x_1, x_2, x_3, x_4);
+return x_5;
 }
 }
 LEAN_EXPORT lean_object* l_Game__World__wDraw_hist__on__turn(lean_object* x_1, lean_object* x_2) {
 _start:
 {
 lean_object* x_3; 
-x_3 = lean_alloc_closure((void*)(l_Game__World__wDraw_hist__on__turn___rarg___boxed), 6, 0);
+x_3 = lean_alloc_closure((void*)(l_Game__World__wDraw_hist__on__turn___rarg___boxed), 4, 0);
 return x_3;
 }
 }
-LEAN_EXPORT lean_object* l_Game__World__wDraw_hist__on__turn___rarg___boxed(lean_object* x_1, lean_object* x_2, lean_object* x_3, lean_object* x_4, lean_object* x_5, lean_object* x_6) {
+LEAN_EXPORT lean_object* l_Game__World__wDraw_hist__on__turn___rarg___boxed(lean_object* x_1, lean_object* x_2, lean_object* x_3, lean_object* x_4) {
 _start:
 {
-lean_object* x_7; 
-x_7 = l_Game__World__wDraw_hist__on__turn___rarg(x_1, x_2, x_3, x_4, x_5, x_6);
-lean_dec(x_6);
-lean_dec(x_3);
-lean_dec(x_2);
+lean_object* x_5; 
+x_5 = l_Game__World__wDraw_hist__on__turn___rarg(x_1, x_2, x_3, x_4);
+lean_dec(x_4);
 lean_dec(x_1);
-return x_7;
+return x_5;
 }
 }
 LEAN_EXPORT lean_object* l_Symm__Game_toGame___elambda__1___rarg(lean_object* x_1, lean_object* x_2, lean_object* x_3, lean_object* x_4) {
@@ -478,103 +460,69 @@ x_3 = lean_alloc_closure((void*)(l_Symm__Game_toGame___rarg), 1, 0);
 return x_3;
 }
 }
-LEAN_EXPORT lean_object* l_Game_hist__on__turn___rarg(lean_object* x_1, lean_object* x_2, lean_object* x_3, lean_object* x_4) {
+LEAN_EXPORT lean_object* l_Game_hist__on__turn___rarg(lean_object* x_1, lean_object* x_2) {
 _start:
 {
-lean_object* x_5; lean_object* x_6; lean_object* x_7; lean_object* x_8; 
-x_5 = lean_ctor_get(x_1, 0);
+lean_object* x_3; lean_object* x_4; lean_object* x_5; lean_object* x_6; 
+x_3 = lean_ctor_get(x_1, 0);
+lean_inc(x_3);
+x_4 = lean_ctor_get(x_1, 1);
+lean_inc(x_4);
+x_5 = lean_ctor_get(x_1, 2);
 lean_inc(x_5);
-x_6 = lean_ctor_get(x_1, 1);
-lean_inc(x_6);
-x_7 = lean_ctor_get(x_1, 2);
-lean_inc(x_7);
 lean_dec(x_1);
-x_8 = l_Game__World_hist__on__turn___rarg(x_5, x_2, x_3, x_6, x_7, x_4);
-lean_dec(x_5);
-return x_8;
+x_6 = l_Game__World_hist__on__turn___rarg(x_3, x_4, x_5, x_2);
+lean_dec(x_3);
+return x_6;
 }
 }
 LEAN_EXPORT lean_object* l_Game_hist__on__turn(lean_object* x_1, lean_object* x_2) {
 _start:
 {
 lean_object* x_3; 
-x_3 = lean_alloc_closure((void*)(l_Game_hist__on__turn___rarg___boxed), 4, 0);
+x_3 = lean_alloc_closure((void*)(l_Game_hist__on__turn___rarg___boxed), 2, 0);
 return x_3;
 }
 }
-LEAN_EXPORT lean_object* l_Game_hist__on__turn___rarg___boxed(lean_object* x_1, lean_object* x_2, lean_object* x_3, lean_object* x_4) {
+LEAN_EXPORT lean_object* l_Game_hist__on__turn___rarg___boxed(lean_object* x_1, lean_object* x_2) {
 _start:
 {
-lean_object* x_5; 
-x_5 = l_Game_hist__on__turn___rarg(x_1, x_2, x_3, x_4);
-lean_dec(x_4);
-lean_dec(x_3);
+lean_object* x_3; 
+x_3 = l_Game_hist__on__turn___rarg(x_1, x_2);
 lean_dec(x_2);
-return x_5;
+return x_3;
 }
 }
-LEAN_EXPORT lean_object* l_Symm__Game__World_hist__on__turn___at_Symm__Game_hist__on__turn___spec__1___rarg(lean_object* x_1, lean_object* x_2, lean_object* x_3, lean_object* x_4, lean_object* x_5, lean_object* x_6) {
+LEAN_EXPORT lean_object* l_Symm__Game_hist__on__turn___rarg(lean_object* x_1, lean_object* x_2) {
 _start:
 {
-lean_object* x_7; lean_object* x_8; 
-x_7 = l_Symm__Game__World_toGame__World___rarg(x_3);
-x_8 = l_Game__World_hist__on__turn___rarg(x_7, x_1, x_2, x_4, x_5, x_6);
-lean_dec(x_7);
-return x_8;
-}
-}
-LEAN_EXPORT lean_object* l_Symm__Game__World_hist__on__turn___at_Symm__Game_hist__on__turn___spec__1(lean_object* x_1, lean_object* x_2, lean_object* x_3) {
-_start:
-{
-lean_object* x_4; 
-x_4 = lean_alloc_closure((void*)(l_Symm__Game__World_hist__on__turn___at_Symm__Game_hist__on__turn___spec__1___rarg___boxed), 6, 0);
-return x_4;
-}
-}
-LEAN_EXPORT lean_object* l_Symm__Game_hist__on__turn___rarg(lean_object* x_1, lean_object* x_2, lean_object* x_3, lean_object* x_4) {
-_start:
-{
-lean_object* x_5; lean_object* x_6; lean_object* x_7; lean_object* x_8; 
-x_5 = lean_ctor_get(x_1, 0);
+lean_object* x_3; lean_object* x_4; lean_object* x_5; lean_object* x_6; 
+x_3 = lean_ctor_get(x_1, 0);
+lean_inc(x_3);
+x_4 = lean_ctor_get(x_1, 1);
+lean_inc(x_4);
+x_5 = lean_ctor_get(x_1, 2);
 lean_inc(x_5);
-x_6 = lean_ctor_get(x_1, 1);
-lean_inc(x_6);
-x_7 = lean_ctor_get(x_1, 2);
-lean_inc(x_7);
 lean_dec(x_1);
-x_8 = l_Symm__Game__World_hist__on__turn___at_Symm__Game_hist__on__turn___spec__1___rarg(x_2, x_3, x_5, x_6, x_7, x_4);
-lean_dec(x_4);
-lean_dec(x_3);
-lean_dec(x_2);
-return x_8;
+x_6 = l_Symm__Game__World_hist__on__turn___rarg(x_3, x_4, x_5, x_2);
+return x_6;
 }
 }
 LEAN_EXPORT lean_object* l_Symm__Game_hist__on__turn(lean_object* x_1, lean_object* x_2) {
 _start:
 {
 lean_object* x_3; 
-x_3 = lean_alloc_closure((void*)(l_Symm__Game_hist__on__turn___rarg), 4, 0);
+x_3 = lean_alloc_closure((void*)(l_Symm__Game_hist__on__turn___rarg___boxed), 2, 0);
 return x_3;
 }
 }
-LEAN_EXPORT lean_object* l_Symm__Game__World_hist__on__turn___at_Symm__Game_hist__on__turn___spec__1___rarg___boxed(lean_object* x_1, lean_object* x_2, lean_object* x_3, lean_object* x_4, lean_object* x_5, lean_object* x_6) {
+LEAN_EXPORT lean_object* l_Symm__Game_hist__on__turn___rarg___boxed(lean_object* x_1, lean_object* x_2) {
 _start:
 {
-lean_object* x_7; 
-x_7 = l_Symm__Game__World_hist__on__turn___at_Symm__Game_hist__on__turn___spec__1___rarg(x_1, x_2, x_3, x_4, x_5, x_6);
-lean_dec(x_6);
+lean_object* x_3; 
+x_3 = l_Symm__Game_hist__on__turn___rarg(x_1, x_2);
 lean_dec(x_2);
-lean_dec(x_1);
-return x_7;
-}
-}
-LEAN_EXPORT lean_object* l_Symm__Game__World_hist__on__turn___at_Symm__Game_hist__on__turn___spec__1___boxed(lean_object* x_1, lean_object* x_2, lean_object* x_3) {
-_start:
-{
-lean_object* x_4; 
-x_4 = l_Symm__Game__World_hist__on__turn___at_Symm__Game_hist__on__turn___spec__1(x_1, x_2, x_3);
-lean_dec(x_3);
-return x_4;
+return x_3;
 }
 }
 LEAN_EXPORT lean_object* l_Game__World_state__from__hist___rarg(lean_object* x_1, lean_object* x_2) {
@@ -632,58 +580,58 @@ x_3 = lean_alloc_closure((void*)(l_Game__World_state__from__hist___rarg), 2, 0);
 return x_3;
 }
 }
-LEAN_EXPORT lean_object* l_Game__World_state__on__turn___rarg(lean_object* x_1, lean_object* x_2, lean_object* x_3, lean_object* x_4, lean_object* x_5, lean_object* x_6) {
+LEAN_EXPORT lean_object* l_Game__World_state__on__turn___rarg(lean_object* x_1, lean_object* x_2, lean_object* x_3, lean_object* x_4) {
 _start:
 {
-lean_object* x_7; uint8_t x_8; 
-x_7 = lean_unsigned_to_nat(0u);
-x_8 = lean_nat_dec_eq(x_6, x_7);
-if (x_8 == 0)
+lean_object* x_5; uint8_t x_6; 
+x_5 = lean_unsigned_to_nat(0u);
+x_6 = lean_nat_dec_eq(x_4, x_5);
+if (x_6 == 0)
 {
-lean_object* x_9; lean_object* x_10; lean_object* x_11; lean_object* x_12; uint8_t x_13; 
-x_9 = lean_unsigned_to_nat(1u);
-x_10 = lean_nat_sub(x_6, x_9);
-lean_inc(x_5);
-lean_inc(x_4);
-x_11 = l_Game__World_hist__on__turn___rarg(x_1, x_2, x_3, x_4, x_5, x_10);
-x_12 = lean_nat_add(x_10, x_9);
+lean_object* x_7; lean_object* x_8; lean_object* x_9; lean_object* x_10; uint8_t x_11; 
+x_7 = lean_unsigned_to_nat(1u);
+x_8 = lean_nat_sub(x_4, x_7);
+lean_inc(x_3);
+lean_inc(x_2);
+x_9 = l_Game__World_hist__on__turn___rarg(x_1, x_2, x_3, x_8);
+x_10 = lean_nat_add(x_8, x_7);
+lean_dec(x_8);
+x_11 = l_instDecidablePredNatTurn__fst(x_10);
 lean_dec(x_10);
-x_13 = l_instDecidablePredNatTurn__fst(x_12);
-lean_dec(x_12);
-if (x_13 == 0)
+if (x_11 == 0)
 {
-lean_object* x_14; lean_object* x_15; lean_object* x_16; 
-lean_dec(x_4);
-x_14 = lean_ctor_get(x_1, 2);
-lean_inc(x_14);
+lean_object* x_12; lean_object* x_13; lean_object* x_14; 
+lean_dec(x_2);
+x_12 = lean_ctor_get(x_1, 2);
+lean_inc(x_12);
 lean_dec(x_1);
-lean_inc(x_11);
-x_15 = lean_apply_3(x_5, x_11, lean_box(0), lean_box(0));
-x_16 = lean_apply_2(x_14, x_11, x_15);
-return x_16;
+lean_inc(x_9);
+x_13 = lean_apply_3(x_3, x_9, lean_box(0), lean_box(0));
+x_14 = lean_apply_2(x_12, x_9, x_13);
+return x_14;
 }
 else
 {
-lean_object* x_17; lean_object* x_18; lean_object* x_19; 
-lean_dec(x_5);
-x_17 = lean_ctor_get(x_1, 1);
-lean_inc(x_17);
+lean_object* x_15; lean_object* x_16; lean_object* x_17; 
+lean_dec(x_3);
+x_15 = lean_ctor_get(x_1, 1);
+lean_inc(x_15);
 lean_dec(x_1);
-lean_inc(x_11);
-x_18 = lean_apply_3(x_4, x_11, lean_box(0), lean_box(0));
-x_19 = lean_apply_2(x_17, x_11, x_18);
-return x_19;
+lean_inc(x_9);
+x_16 = lean_apply_3(x_2, x_9, lean_box(0), lean_box(0));
+x_17 = lean_apply_2(x_15, x_9, x_16);
+return x_17;
 }
 }
 else
 {
-lean_object* x_20; 
-lean_dec(x_5);
-lean_dec(x_4);
-x_20 = lean_ctor_get(x_1, 0);
-lean_inc(x_20);
+lean_object* x_18; 
+lean_dec(x_3);
+lean_dec(x_2);
+x_18 = lean_ctor_get(x_1, 0);
+lean_inc(x_18);
 lean_dec(x_1);
-return x_20;
+return x_18;
 }
 }
 }
@@ -691,291 +639,107 @@ LEAN_EXPORT lean_object* l_Game__World_state__on__turn(lean_object* x_1, lean_ob
 _start:
 {
 lean_object* x_3; 
-x_3 = lean_alloc_closure((void*)(l_Game__World_state__on__turn___rarg___boxed), 6, 0);
+x_3 = lean_alloc_closure((void*)(l_Game__World_state__on__turn___rarg___boxed), 4, 0);
 return x_3;
 }
 }
-LEAN_EXPORT lean_object* l_Game__World_state__on__turn___rarg___boxed(lean_object* x_1, lean_object* x_2, lean_object* x_3, lean_object* x_4, lean_object* x_5, lean_object* x_6) {
+LEAN_EXPORT lean_object* l_Game__World_state__on__turn___rarg___boxed(lean_object* x_1, lean_object* x_2, lean_object* x_3, lean_object* x_4) {
 _start:
 {
-lean_object* x_7; 
-x_7 = l_Game__World_state__on__turn___rarg(x_1, x_2, x_3, x_4, x_5, x_6);
-lean_dec(x_6);
-lean_dec(x_3);
-lean_dec(x_2);
-return x_7;
+lean_object* x_5; 
+x_5 = l_Game__World_state__on__turn___rarg(x_1, x_2, x_3, x_4);
+lean_dec(x_4);
+return x_5;
 }
 }
-LEAN_EXPORT lean_object* l_Symm__Game__World_state__on__turn___rarg(lean_object* x_1, lean_object* x_2, lean_object* x_3, lean_object* x_4, lean_object* x_5, lean_object* x_6) {
+LEAN_EXPORT lean_object* l_Symm__Game__World_state__on__turn___rarg(lean_object* x_1, lean_object* x_2, lean_object* x_3, lean_object* x_4) {
 _start:
 {
-lean_object* x_7; lean_object* x_8; 
-x_7 = l_Symm__Game__World_toGame__World___rarg(x_1);
-x_8 = l_Game__World_state__on__turn___rarg(x_7, x_2, x_3, x_4, x_5, x_6);
-return x_8;
+lean_object* x_5; lean_object* x_6; 
+x_5 = l_Symm__Game__World_toGame__World___rarg(x_1);
+x_6 = l_Game__World_state__on__turn___rarg(x_5, x_2, x_3, x_4);
+return x_6;
 }
 }
 LEAN_EXPORT lean_object* l_Symm__Game__World_state__on__turn(lean_object* x_1, lean_object* x_2) {
 _start:
 {
 lean_object* x_3; 
-x_3 = lean_alloc_closure((void*)(l_Symm__Game__World_state__on__turn___rarg___boxed), 6, 0);
+x_3 = lean_alloc_closure((void*)(l_Symm__Game__World_state__on__turn___rarg___boxed), 4, 0);
 return x_3;
 }
 }
-LEAN_EXPORT lean_object* l_Symm__Game__World_state__on__turn___rarg___boxed(lean_object* x_1, lean_object* x_2, lean_object* x_3, lean_object* x_4, lean_object* x_5, lean_object* x_6) {
+LEAN_EXPORT lean_object* l_Symm__Game__World_state__on__turn___rarg___boxed(lean_object* x_1, lean_object* x_2, lean_object* x_3, lean_object* x_4) {
 _start:
 {
-lean_object* x_7; 
-x_7 = l_Symm__Game__World_state__on__turn___rarg(x_1, x_2, x_3, x_4, x_5, x_6);
-lean_dec(x_6);
-lean_dec(x_3);
-lean_dec(x_2);
-return x_7;
+lean_object* x_5; 
+x_5 = l_Symm__Game__World_state__on__turn___rarg(x_1, x_2, x_3, x_4);
+lean_dec(x_4);
+return x_5;
 }
 }
-LEAN_EXPORT lean_object* l_Game__World_state__on__turn___at_Game_state__on__turn___spec__1___rarg(lean_object* x_1, lean_object* x_2, lean_object* x_3, lean_object* x_4, lean_object* x_5, lean_object* x_6) {
+LEAN_EXPORT lean_object* l_Game_state__on__turn___rarg(lean_object* x_1, lean_object* x_2) {
 _start:
 {
-lean_object* x_7; uint8_t x_8; 
-x_7 = lean_unsigned_to_nat(0u);
-x_8 = lean_nat_dec_eq(x_6, x_7);
-if (x_8 == 0)
-{
-lean_object* x_9; lean_object* x_10; lean_object* x_11; lean_object* x_12; uint8_t x_13; 
-x_9 = lean_unsigned_to_nat(1u);
-x_10 = lean_nat_sub(x_6, x_9);
-lean_inc(x_5);
+lean_object* x_3; lean_object* x_4; lean_object* x_5; lean_object* x_6; 
+x_3 = lean_ctor_get(x_1, 0);
+lean_inc(x_3);
+x_4 = lean_ctor_get(x_1, 1);
 lean_inc(x_4);
-x_11 = l_Game__World_hist__on__turn___rarg(x_3, x_1, x_2, x_4, x_5, x_10);
-x_12 = lean_nat_add(x_10, x_9);
-lean_dec(x_10);
-x_13 = l_instDecidablePredNatTurn__fst(x_12);
-lean_dec(x_12);
-if (x_13 == 0)
-{
-lean_object* x_14; lean_object* x_15; lean_object* x_16; 
-lean_dec(x_4);
-x_14 = lean_ctor_get(x_3, 2);
-lean_inc(x_14);
-lean_dec(x_3);
-lean_inc(x_11);
-x_15 = lean_apply_3(x_5, x_11, lean_box(0), lean_box(0));
-x_16 = lean_apply_2(x_14, x_11, x_15);
-return x_16;
-}
-else
-{
-lean_object* x_17; lean_object* x_18; lean_object* x_19; 
-lean_dec(x_5);
-x_17 = lean_ctor_get(x_3, 1);
-lean_inc(x_17);
-lean_dec(x_3);
-lean_inc(x_11);
-x_18 = lean_apply_3(x_4, x_11, lean_box(0), lean_box(0));
-x_19 = lean_apply_2(x_17, x_11, x_18);
-return x_19;
-}
-}
-else
-{
-lean_object* x_20; 
-lean_dec(x_5);
-lean_dec(x_4);
-x_20 = lean_ctor_get(x_3, 0);
-lean_inc(x_20);
-lean_dec(x_3);
-return x_20;
-}
-}
-}
-LEAN_EXPORT lean_object* l_Game__World_state__on__turn___at_Game_state__on__turn___spec__1(lean_object* x_1, lean_object* x_2, lean_object* x_3) {
-_start:
-{
-lean_object* x_4; 
-x_4 = lean_alloc_closure((void*)(l_Game__World_state__on__turn___at_Game_state__on__turn___spec__1___rarg___boxed), 6, 0);
-return x_4;
-}
-}
-LEAN_EXPORT lean_object* l_Game_state__on__turn___rarg(lean_object* x_1, lean_object* x_2, lean_object* x_3, lean_object* x_4) {
-_start:
-{
-lean_object* x_5; lean_object* x_6; lean_object* x_7; lean_object* x_8; 
-x_5 = lean_ctor_get(x_1, 0);
+x_5 = lean_ctor_get(x_1, 2);
 lean_inc(x_5);
-x_6 = lean_ctor_get(x_1, 1);
-lean_inc(x_6);
-x_7 = lean_ctor_get(x_1, 2);
-lean_inc(x_7);
 lean_dec(x_1);
-x_8 = l_Game__World_state__on__turn___at_Game_state__on__turn___spec__1___rarg(x_2, x_3, x_5, x_6, x_7, x_4);
-lean_dec(x_4);
-lean_dec(x_3);
-lean_dec(x_2);
-return x_8;
+x_6 = l_Game__World_state__on__turn___rarg(x_3, x_4, x_5, x_2);
+return x_6;
 }
 }
 LEAN_EXPORT lean_object* l_Game_state__on__turn(lean_object* x_1, lean_object* x_2) {
 _start:
 {
 lean_object* x_3; 
-x_3 = lean_alloc_closure((void*)(l_Game_state__on__turn___rarg), 4, 0);
+x_3 = lean_alloc_closure((void*)(l_Game_state__on__turn___rarg___boxed), 2, 0);
 return x_3;
 }
 }
-LEAN_EXPORT lean_object* l_Game__World_state__on__turn___at_Game_state__on__turn___spec__1___rarg___boxed(lean_object* x_1, lean_object* x_2, lean_object* x_3, lean_object* x_4, lean_object* x_5, lean_object* x_6) {
-_start:
-{
-lean_object* x_7; 
-x_7 = l_Game__World_state__on__turn___at_Game_state__on__turn___spec__1___rarg(x_1, x_2, x_3, x_4, x_5, x_6);
-lean_dec(x_6);
-lean_dec(x_2);
-lean_dec(x_1);
-return x_7;
-}
-}
-LEAN_EXPORT lean_object* l_Game__World_state__on__turn___at_Game_state__on__turn___spec__1___boxed(lean_object* x_1, lean_object* x_2, lean_object* x_3) {
-_start:
-{
-lean_object* x_4; 
-x_4 = l_Game__World_state__on__turn___at_Game_state__on__turn___spec__1(x_1, x_2, x_3);
-lean_dec(x_3);
-return x_4;
-}
-}
-LEAN_EXPORT lean_object* l_Game__World_state__on__turn___at_Symm__Game_state__on__turn___spec__2___rarg(lean_object* x_1, lean_object* x_2, lean_object* x_3, lean_object* x_4, lean_object* x_5, lean_object* x_6) {
-_start:
-{
-lean_object* x_7; uint8_t x_8; 
-x_7 = lean_unsigned_to_nat(0u);
-x_8 = lean_nat_dec_eq(x_6, x_7);
-if (x_8 == 0)
-{
-lean_object* x_9; lean_object* x_10; lean_object* x_11; lean_object* x_12; uint8_t x_13; 
-x_9 = lean_unsigned_to_nat(1u);
-x_10 = lean_nat_sub(x_6, x_9);
-lean_inc(x_5);
-lean_inc(x_4);
-x_11 = l_Game__World_hist__on__turn___rarg(x_3, x_1, x_2, x_4, x_5, x_10);
-x_12 = lean_nat_add(x_10, x_9);
-lean_dec(x_10);
-x_13 = l_instDecidablePredNatTurn__fst(x_12);
-lean_dec(x_12);
-if (x_13 == 0)
-{
-lean_object* x_14; lean_object* x_15; lean_object* x_16; 
-lean_dec(x_4);
-x_14 = lean_ctor_get(x_3, 2);
-lean_inc(x_14);
-lean_dec(x_3);
-lean_inc(x_11);
-x_15 = lean_apply_3(x_5, x_11, lean_box(0), lean_box(0));
-x_16 = lean_apply_2(x_14, x_11, x_15);
-return x_16;
-}
-else
-{
-lean_object* x_17; lean_object* x_18; lean_object* x_19; 
-lean_dec(x_5);
-x_17 = lean_ctor_get(x_3, 1);
-lean_inc(x_17);
-lean_dec(x_3);
-lean_inc(x_11);
-x_18 = lean_apply_3(x_4, x_11, lean_box(0), lean_box(0));
-x_19 = lean_apply_2(x_17, x_11, x_18);
-return x_19;
-}
-}
-else
-{
-lean_object* x_20; 
-lean_dec(x_5);
-lean_dec(x_4);
-x_20 = lean_ctor_get(x_3, 0);
-lean_inc(x_20);
-lean_dec(x_3);
-return x_20;
-}
-}
-}
-LEAN_EXPORT lean_object* l_Game__World_state__on__turn___at_Symm__Game_state__on__turn___spec__2(lean_object* x_1, lean_object* x_2, lean_object* x_3) {
-_start:
-{
-lean_object* x_4; 
-x_4 = lean_alloc_closure((void*)(l_Game__World_state__on__turn___at_Symm__Game_state__on__turn___spec__2___rarg___boxed), 6, 0);
-return x_4;
-}
-}
-LEAN_EXPORT lean_object* l_Symm__Game__World_state__on__turn___at_Symm__Game_state__on__turn___spec__1___rarg(lean_object* x_1, lean_object* x_2, lean_object* x_3, lean_object* x_4, lean_object* x_5, lean_object* x_6, lean_object* x_7) {
-_start:
-{
-lean_object* x_8; lean_object* x_9; 
-lean_dec(x_1);
-x_8 = l_Symm__Game__World_toGame__World___rarg(x_4);
-x_9 = l_Game__World_state__on__turn___at_Symm__Game_state__on__turn___spec__2___rarg(x_2, x_3, x_8, x_5, x_6, x_7);
-lean_dec(x_3);
-lean_dec(x_2);
-return x_9;
-}
-}
-LEAN_EXPORT lean_object* l_Symm__Game__World_state__on__turn___at_Symm__Game_state__on__turn___spec__1(lean_object* x_1, lean_object* x_2) {
+LEAN_EXPORT lean_object* l_Game_state__on__turn___rarg___boxed(lean_object* x_1, lean_object* x_2) {
 _start:
 {
 lean_object* x_3; 
-x_3 = lean_alloc_closure((void*)(l_Symm__Game__World_state__on__turn___at_Symm__Game_state__on__turn___spec__1___rarg___boxed), 7, 0);
+x_3 = l_Game_state__on__turn___rarg(x_1, x_2);
+lean_dec(x_2);
 return x_3;
 }
 }
-LEAN_EXPORT lean_object* l_Symm__Game_state__on__turn___rarg(lean_object* x_1, lean_object* x_2, lean_object* x_3, lean_object* x_4) {
+LEAN_EXPORT lean_object* l_Symm__Game_state__on__turn___rarg(lean_object* x_1, lean_object* x_2) {
 _start:
 {
-lean_object* x_5; lean_object* x_6; lean_object* x_7; lean_object* x_8; 
-x_5 = lean_ctor_get(x_1, 0);
+lean_object* x_3; lean_object* x_4; lean_object* x_5; lean_object* x_6; 
+x_3 = lean_ctor_get(x_1, 0);
+lean_inc(x_3);
+x_4 = lean_ctor_get(x_1, 1);
+lean_inc(x_4);
+x_5 = lean_ctor_get(x_1, 2);
 lean_inc(x_5);
-x_6 = lean_ctor_get(x_1, 1);
-lean_inc(x_6);
-x_7 = lean_ctor_get(x_1, 2);
-lean_inc(x_7);
-x_8 = l_Symm__Game__World_state__on__turn___at_Symm__Game_state__on__turn___spec__1___rarg(x_1, x_2, x_3, x_5, x_6, x_7, x_4);
-lean_dec(x_4);
-return x_8;
+lean_dec(x_1);
+x_6 = l_Symm__Game__World_state__on__turn___rarg(x_3, x_4, x_5, x_2);
+return x_6;
 }
 }
 LEAN_EXPORT lean_object* l_Symm__Game_state__on__turn(lean_object* x_1, lean_object* x_2) {
 _start:
 {
 lean_object* x_3; 
-x_3 = lean_alloc_closure((void*)(l_Symm__Game_state__on__turn___rarg), 4, 0);
+x_3 = lean_alloc_closure((void*)(l_Symm__Game_state__on__turn___rarg___boxed), 2, 0);
 return x_3;
 }
 }
-LEAN_EXPORT lean_object* l_Game__World_state__on__turn___at_Symm__Game_state__on__turn___spec__2___rarg___boxed(lean_object* x_1, lean_object* x_2, lean_object* x_3, lean_object* x_4, lean_object* x_5, lean_object* x_6) {
+LEAN_EXPORT lean_object* l_Symm__Game_state__on__turn___rarg___boxed(lean_object* x_1, lean_object* x_2) {
 _start:
 {
-lean_object* x_7; 
-x_7 = l_Game__World_state__on__turn___at_Symm__Game_state__on__turn___spec__2___rarg(x_1, x_2, x_3, x_4, x_5, x_6);
-lean_dec(x_6);
+lean_object* x_3; 
+x_3 = l_Symm__Game_state__on__turn___rarg(x_1, x_2);
 lean_dec(x_2);
-lean_dec(x_1);
-return x_7;
-}
-}
-LEAN_EXPORT lean_object* l_Game__World_state__on__turn___at_Symm__Game_state__on__turn___spec__2___boxed(lean_object* x_1, lean_object* x_2, lean_object* x_3) {
-_start:
-{
-lean_object* x_4; 
-x_4 = l_Game__World_state__on__turn___at_Symm__Game_state__on__turn___spec__2(x_1, x_2, x_3);
-lean_dec(x_3);
-return x_4;
-}
-}
-LEAN_EXPORT lean_object* l_Symm__Game__World_state__on__turn___at_Symm__Game_state__on__turn___spec__1___rarg___boxed(lean_object* x_1, lean_object* x_2, lean_object* x_3, lean_object* x_4, lean_object* x_5, lean_object* x_6, lean_object* x_7) {
-_start:
-{
-lean_object* x_8; 
-x_8 = l_Symm__Game__World_state__on__turn___at_Symm__Game_state__on__turn___spec__1___rarg(x_1, x_2, x_3, x_4, x_5, x_6, x_7);
-lean_dec(x_7);
-return x_8;
+return x_3;
 }
 }
 lean_object* initialize_Init(uint8_t builtin, lean_object*);
