Games/gameLib/Termination.lean
@@ -8,20 +8,31 @@ import Games.gameLib.Basic
 
 
 
+
+/-
+This file defines notions surrounding those of termination of games and winng strategies.
+The big picture is:
+- `Turn_isWL` defines what it means for a turn to be terminal
+- `isWL` defines what it means for a `Game_World` having all its possible games terminate
+- `fst_win` and `snd_win` define what it means for a game to be won by the corresponding player
+- `is_fst_win` and `is_snd_win` define what it means for either player to have a winning strategy.
+
+-/
+
+
 /--
 A turn is win or lose (WL) if the `hist_on_turn` at that turn satisfies
 one of the predicates that decide if a player wins at that stage in the game.
 -/
 inductive Game_World.Turn_isWL (g : Game_World α β)
-  [DecidablePred (g.fst_win_states)] [DecidablePred (g.snd_win_states )]
+
   (f_strat : g.fStrategy) (s_strat : g.sStrategy) (turn : ℕ) : Prop where
   | wf : g.fst_win_states (g.hist_on_turn f_strat s_strat turn) → g.Turn_isWL f_strat s_strat turn
   | ws : g.snd_win_states  (g.hist_on_turn f_strat s_strat turn) → g.Turn_isWL f_strat s_strat turn
 
 def Symm_Game_World.Turn_isWL (g : Symm_Game_World α β)
-  [DecidablePred (g.fst_win_states)] [DecidablePred (g.snd_win_states )]
   (f_strat : g.fStrategy) (s_strat : g.sStrategy) (turn : ℕ) : Prop :=
-  @Game_World.Turn_isWL _ _ (g.toGame_World) (by rwa [g.toGame_World_fst_win]) (by rwa [g.toGame_World_snd_win]) f_strat s_strat turn
+  Game_World.Turn_isWL (g.toGame_World) f_strat s_strat turn
 
 /--
 A `Game_World` is win or lose (WL) if for any pair of strategies the players
@@ -31,35 +42,33 @@ these strategies.
 In particular, all games terminate.
 -/
 def Game_World.isWL (g : Game_World α β)
-  [DecidablePred (g.fst_win_states)] [DecidablePred (g.snd_win_states )]: Prop :=
+  : Prop :=
   ∀ (f_strat : g.fStrategy), ∀ (s_strat : g.sStrategy),
   ∃ turn, g.Turn_isWL f_strat s_strat turn
 
 def Symm_Game_World.isWL (g : Symm_Game_World α β)
-  [DecidablePred (g.fst_win_states)] [DecidablePred (g.snd_win_states )]: Prop :=
+  : Prop :=
   ∀ (f_strat : g.fStrategy), ∀ (s_strat : g.sStrategy),
   ∃ turn, g.Turn_isWL f_strat s_strat turn
 
 
 def Game_World.state_on_turn_neutral (g : Game_World α β)
-  [DecidablePred (g.fst_win_states)] [DecidablePred (g.snd_win_states )]
   (f_strat : g.fStrategy) (s_strat : g.sStrategy) (turn : ℕ) : Prop :=
   ¬ g.Turn_isWL f_strat s_strat turn
 
 def Symm_Game_World.state_on_turn_neutral (g : Symm_Game_World α β)
-  [DecidablePred (g.fst_win_states)] [DecidablePred (g.snd_win_states )]
+
   (f_strat : g.fStrategy) (s_strat : g.sStrategy) (turn : ℕ) : Prop :=
-  @Game_World.state_on_turn_neutral _ _  (g.toGame_World) (by rwa [g.toGame_World_fst_win]) (by rwa [g.toGame_World_snd_win]) f_strat s_strat turn
+  Game_World.state_on_turn_neutral (g.toGame_World) f_strat s_strat turn
 
 def Game.state_on_turn_neutral (g : Game α β)
-  [DecidablePred (g.fst_win_states)] [DecidablePred (g.snd_win_states )]
+
   (turn : ℕ) : Prop :=
   g.toGame_World.state_on_turn_neutral g.fst_strat g.snd_strat turn
 
 def Symm_Game.state_on_turn_neutral (g : Symm_Game α β)
-  [DecidablePred (g.fst_win_states)] [DecidablePred (g.snd_win_states )]
   (turn : ℕ) : Prop :=
-  @Game.state_on_turn_neutral _ _ g.toGame (by rwa [g.toGame_fst_win]) (by rwa [g.toGame_snd_win]) turn
+  Game.state_on_turn_neutral g.toGame turn
 
 /-- The game is won by the first player if there is a turn such that
 all prior turns were neutral, and the first winning predicate is satisfied
@@ -68,7 +77,7 @@ at that turn
 In particular, the game terminates.
 -/
 def Game.fst_win (g : Game α β)
-  [DecidablePred (g.fst_win_states)] [DecidablePred (g.snd_win_states )] : Prop :=
+   : Prop :=
   ∃ turn : ℕ, g.fst_win_states (g.hist_on_turn turn) ∧ (∀ t < turn, g.state_on_turn_neutral t)
 
 /-- The game is won by the second player if there is a turn such that
@@ -78,16 +87,16 @@ at that turn
 In particular, the game terminates.
 -/
 def Game.snd_win (g : Game α β)
-  [DecidablePred (g.fst_win_states)] [DecidablePred (g.snd_win_states )] : Prop :=
+   : Prop :=
   ∃ turn : ℕ, g.snd_win_states (g.hist_on_turn turn) ∧ (∀ t < turn, g.state_on_turn_neutral t)
 
 def Symm_Game.fst_win (g : Symm_Game α β)
-  [DecidablePred (g.fst_win_states)] [DecidablePred (g.snd_win_states )] : Prop :=
-  @Game.fst_win _ _ g.toGame (by rwa [g.toGame_fst_win]) (by rwa [g.toGame_snd_win])
+  : Prop :=
+  Game.fst_win g.toGame
 
 def Symm_Game.snd_win (g : Symm_Game α β)
-  [DecidablePred (g.fst_win_states)] [DecidablePred (g.snd_win_states )] : Prop :=
-  @Game.snd_win _ _ g.toGame (by rwa [g.toGame_fst_win]) (by rwa [g.toGame_snd_win])
+   : Prop :=
+  Game.snd_win g.toGame
 
 
 /--
@@ -98,7 +107,7 @@ won by the first player.
 In particular, all games terminate.
 -/
 def Game_World.is_fst_win (g : Game_World α β)
-  [DecidablePred (g.fst_win_states)] [DecidablePred (g.snd_win_states )] : Prop :=
+   : Prop :=
   ∃ ws : g.fStrategy, ∀ snd_s : g.sStrategy,
   ({g with fst_strat := ws, snd_strat := snd_s} : Game α β).fst_win
 
@@ -111,33 +120,31 @@ won by the second player.
 In particular, all games terminate.
 -/
 def Game_World.is_snd_win (g : Game_World α β)
-  [DecidablePred (g.fst_win_states)] [DecidablePred (g.snd_win_states )] : Prop :=
+   : Prop :=
   ∃ ws : g.sStrategy, ∀ snd_s : g.fStrategy,
   ({g with snd_strat := ws, fst_strat := snd_s} : Game α β).snd_win
 
 def Symm_Game_World.is_fst_win (g : Symm_Game_World α β)
-  [DecidablePred (g.fst_win_states)] [DecidablePred (g.snd_win_states )] : Prop :=
-  @Game_World.is_fst_win _ _ g.toGame_World (by rwa [g.toGame_World_fst_win]) (by rwa [g.toGame_World_snd_win])
+   : Prop :=
+  Game_World.is_fst_win g.toGame_World
 
 def Symm_Game_World.is_snd_win (g : Symm_Game_World α β)
-  [DecidablePred (g.fst_win_states)] [DecidablePred (g.snd_win_states )]: Prop :=
-  @Game_World.is_snd_win _ _ g.toGame_World (by rwa [g.toGame_World_fst_win]) (by rwa [g.toGame_World_snd_win])
+  : Prop :=
+  Game_World.is_snd_win g.toGame_World
 
 /--
 The `Game_World` has a winning strategy if it has one for one of the players.
 -/
 inductive Game_World.has_WL (g : Game_World α β)
-  [DecidablePred (g.fst_win_states)] [DecidablePred (g.snd_win_states )] : Prop where
+   : Prop where
   | wf (h : g.is_fst_win)
   | ws (h : g.is_snd_win)
 
-def Symm_Game_World.has_WL (g : Symm_Game_World α β)
-  [DecidablePred (g.fst_win_states)] [DecidablePred (g.snd_win_states )] :=
-  @Game_World.has_WL _ _ g.toGame_World (by rwa [g.toGame_World_fst_win]) (by rwa [g.toGame_World_snd_win])
+def Symm_Game_World.has_WL (g : Symm_Game_World α β) :=
+  Game_World.has_WL g.toGame_World
 
 
 lemma Game_World.state_on_turn_neutral_State_from_history_neutral (g : Game_World α β)
-  [DecidablePred (g.fst_win_states)] [DecidablePred (g.snd_win_states )]
   (f_strat : g.fStrategy) (s_strat : g.sStrategy) (turn : ℕ) :
   g.state_on_turn_neutral f_strat s_strat turn ↔
   g.hist_neutral (g.hist_on_turn f_strat s_strat turn).val :=
@@ -158,7 +165,6 @@ lemma Game_World.state_on_turn_neutral_State_from_history_neutral (g : Game_Worl
 
 
 inductive Game_World_wDraw.Turn_isWLD (g : Game_World_wDraw α β)
-  [DecidablePred (g.fst_win_states)] [DecidablePred (g.snd_win_states )]
   (f_strat : g.fStrategy) (s_strat : g.sStrategy) (turn : ℕ) : Prop where
 | wf : g.fst_win_states (g.hist_on_turn f_strat s_strat turn) → g.Turn_isWLD f_strat s_strat turn
 | ws : g.snd_win_states (g.hist_on_turn f_strat s_strat turn) → g.Turn_isWLD f_strat s_strat turn
@@ -166,71 +172,71 @@ inductive Game_World_wDraw.Turn_isWLD (g : Game_World_wDraw α β)
 
 
 def Game_World_wDraw.isWLD (g : Game_World_wDraw α β)
-  [DecidablePred (g.fst_win_states)] [DecidablePred (g.snd_win_states )] : Prop :=
+   : Prop :=
   ∀ (f_strat : g.fStrategy), ∀ (s_strat : g.sStrategy),
   ∃ turn, g.Turn_isWLD f_strat s_strat turn
 
 
 def Game_World_wDraw.state_on_turn_neutral (g : Game_World_wDraw α β)
-  [DecidablePred (g.fst_win_states)] [DecidablePred (g.snd_win_states )]
+
   (f_strat : g.fStrategy) (s_strat : g.sStrategy) (turn : ℕ) : Prop :=
   ¬ g.Turn_isWLD f_strat s_strat turn
 
 
 def Game_wDraw.state_on_turn_neutral (g : Game_wDraw α β)
-  [DecidablePred (g.fst_win_states)] [DecidablePred (g.snd_win_states )] (turn : ℕ) : Prop :=
+   (turn : ℕ) : Prop :=
   g.toGame_World_wDraw.state_on_turn_neutral g.fst_strat g.snd_strat turn
 
 
 def Game_wDraw.fst_win  {α β : Type _} (g : Game_wDraw α β)
-  [DecidablePred (g.fst_win_states)] [DecidablePred (g.snd_win_states )] : Prop :=
+   : Prop :=
   ∃ turn : ℕ, g.fst_win_states (g.hist_on_turn g.fst_strat g.snd_strat turn) ∧
     (∀ t < turn, g.state_on_turn_neutral t)
 
 def Game_wDraw.snd_win  {α β : Type _} (g : Game_wDraw α β)
-  [DecidablePred (g.fst_win_states)] [DecidablePred (g.snd_win_states )] : Prop :=
+   : Prop :=
   ∃ turn : ℕ, g.snd_win_states (g.hist_on_turn g.fst_strat g.snd_strat turn) ∧
     (∀ t < turn, g.state_on_turn_neutral t)
 
 def Game_wDraw.draw  {α β : Type _} (g : Game_wDraw α β)
-  [DecidablePred (g.fst_win_states)] [DecidablePred (g.snd_win_states )] : Prop :=
+   : Prop :=
   ∃ turn : ℕ, g.draw_states (g.hist_on_turn g.fst_strat g.snd_strat turn) ∧
     (∀ t < turn, g.state_on_turn_neutral t)
 
 
 def Game_World_wDraw.is_fst_win  {α β : Type _} (g : Game_World_wDraw α β)
-  [DecidablePred (g.fst_win_states)] [DecidablePred (g.snd_win_states )] : Prop :=
+   : Prop :=
   ∃ ws : g.fStrategy, ∀ snd_s : g.sStrategy,
   ({g with fst_strat := ws, snd_strat := snd_s} : Game_wDraw α β).fst_win
 
 def Game_World_wDraw.is_snd_win  {α β : Type _} (g : Game_World_wDraw α β)
-  [DecidablePred (g.fst_win_states)] [DecidablePred (g.snd_win_states )] : Prop :=
+   : Prop :=
   ∃ ws : g.sStrategy, ∀ snd_s : g.fStrategy,
   ({g with snd_strat := ws, fst_strat := snd_s} : Game_wDraw α β).fst_win
 
 def Game_World_wDraw.is_draw_fst  {α β : Type _} (g : Game_World_wDraw α β)
-  [DecidablePred (g.fst_win_states)] [DecidablePred (g.snd_win_states )] : Prop :=
+   : Prop :=
   ∃ ws : g.fStrategy, ∀ snd_s : g.sStrategy,
   ({g with fst_strat := ws, snd_strat := snd_s} : Game_wDraw α β).draw
 
 def Game_World_wDraw.is_draw_snd  {α β : Type _} (g : Game_World_wDraw α β)
-  [DecidablePred (g.fst_win_states)] [DecidablePred (g.snd_win_states )] : Prop :=
+   : Prop :=
   ∃ ws : g.sStrategy, ∀ snd_s : g.fStrategy,
   ({g with snd_strat := ws, fst_strat := snd_s} : Game_wDraw α β).draw
 
 def Game_World_wDraw.is_draw {α β : Type _} (g : Game_World_wDraw α β)
-  [DecidablePred (g.fst_win_states)] [DecidablePred (g.snd_win_states )]: Prop :=
+  : Prop :=
   g.is_draw_fst ∨ g.is_draw_snd
 
 inductive Game_World_wDraw.has_WLD (g : Game_World_wDraw α β)
-  [DecidablePred (g.fst_win_states)] [DecidablePred (g.snd_win_states )] : Prop where
+   : Prop where
   | wf (h : g.is_fst_win)
   | ws (h : g.is_snd_win)
   | draw (h : g.is_draw)
 
 
 lemma Game_World_wDraw.state_on_turn_neutral_State_from_history_neutral (g : Game_World_wDraw α β)
-  [DecidablePred (g.fst_win_states)] [DecidablePred (g.snd_win_states )]
+
   (f_strat : g.fStrategy) (s_strat : g.sStrategy) (turn : ℕ) :
   g.state_on_turn_neutral f_strat s_strat turn ↔
   g.hist_neutral (g.hist_on_turn f_strat s_strat turn).val :=
@@ -251,13 +257,13 @@ lemma Game_World_wDraw.state_on_turn_neutral_State_from_history_neutral (g : Gam
 
 
 def Game_World_wDraw.is_draw_at_worst_fst {α β : Type _} (g : Game_World_wDraw α β)
-  [DecidablePred (g.fst_win_states)] [DecidablePred (g.snd_win_states )] : Prop :=
+   : Prop :=
   ∃ ws : g.fStrategy, ∀ snd_s : g.sStrategy,
   ({g with fst_strat := ws, snd_strat := snd_s} : Game_wDraw α β).fst_win ∨
   ({g with fst_strat := ws, snd_strat := snd_s} : Game_wDraw  α β).draw
 
 def Game_World_wDraw.is_draw_at_worst_snd {α β : Type _} (g : Game_World_wDraw α β)
-  [DecidablePred (g.fst_win_states)] [DecidablePred (g.snd_win_states )] : Prop :=
+   : Prop :=
   ∃ ws : g.sStrategy, ∀ fst_s : g.fStrategy,
   ({g with fst_strat := fst_s, snd_strat := ws} : Game_wDraw α β).snd_win ∨
   ({g with fst_strat := fst_s, snd_strat := ws} : Game_wDraw  α β).draw
